WIP

src/lowparse/LowParse.Low.Tac.Sum.fst
@@ -34,3 +34,269 @@ let sum_accessor_ext (ty: term) : Tac unit =
           )
         )
       ]
+
+(* Construct a sum type parser from a F* sum type *)
+
+noextract
+let get_name_and_ctors (s: term) : Tac (name & list ctor) =
+  let e = top_env () in
+  let typename = match inspect s with
+  | Tv_FVar fv -> inspect_fv fv
+  | _ -> fail "not a type name"
+  in
+  match lookup_typ e typename with
+  | None -> fail "type not found"
+  | Some se ->
+    begin match inspect_sigelt se with
+    | Sg_Inductive name _ _ _ constructors -> name, constructors
+    | _ -> fail "not an inductive type"
+    end
+
+noextract
+let typ_eq_name (t: typ) (n: name) : Tac bool =
+  match inspect t with
+  | Tv_FVar fv ->
+    (inspect_fv fv `compare_name` n) = FStar.Order.Eq
+  | _ -> false
+
+noextract
+noeq
+type constr_aux_t = {
+  constr_aux_payload_typ: typ;
+  constr_synth_pattern: pattern;
+  constr_synth_args: list argv;
+  constr_synth_recip_bvs: list bv;
+  constr_synth_recip_body: term;
+}
+
+let get_fv (tm: term) : Tac fv =
+  match inspect tm with
+  | Tv_FVar fv -> fv
+  | _ -> fail "not an fv"
+
+noextract
+let rec mk_constr_aux (iname: name) (t: typ) : Tac constr_aux_t =
+  if t `typ_eq_name` iname
+  then {
+    constr_aux_payload_typ = (`unit);
+    constr_synth_recip_bvs = [];
+    constr_synth_recip_body = (`());
+    constr_synth_pattern = Pat_Constant C_Unit;
+    constr_synth_args = [];
+  }
+  else match inspect t with
+  | Tv_Arrow bv c ->
+    let (bv, _) = inspect_binder bv in
+    let arg_t = (inspect_bv bv).bv_sort in
+    begin match inspect_comp c with
+    | C_Total ret _ ->
+      if ret `typ_eq_name` iname
+      then
+        let b = fresh_bv ret in
+        let br = fresh_bv ret in
+        {
+          constr_aux_payload_typ = ret;
+          constr_synth_recip_bvs = [b];
+          constr_synth_recip_body = pack (Tv_BVar b);
+          constr_synth_pattern = Pat_Var br;
+          constr_synth_args = [pack (Tv_BVar br), Q_Explicit];
+        }
+      else
+        let j = mk_constr_aux iname ret in
+        let b = fresh_bv ret in
+        let br = fresh_bv ret in
+        {
+          constr_aux_payload_typ = mk_app (`tuple2) [arg_t, Q_Explicit; j.constr_aux_payload_typ, Q_Explicit];
+          constr_synth_recip_bvs = b :: j.constr_synth_recip_bvs;
+          constr_synth_recip_body = mk_app (`Mktuple2) [
+            ret, Q_Implicit;
+            j.constr_aux_payload_typ, Q_Implicit;
+            pack (Tv_BVar b), Q_Explicit;
+            j.constr_synth_recip_body, Q_Explicit;
+          ];
+          constr_synth_pattern = Pat_Cons (get_fv (`Mktuple2)) [Pat_Var br, true; j.constr_synth_pattern, true];
+          constr_synth_args = (pack (Tv_BVar br), Q_Explicit) :: j.constr_synth_args;
+        }
+    | _ -> fail "not a Tot constructor"
+    end
+  | _ -> fail "not an arrow constructor"
+
+noextract
+noeq
+type constr_t = {
+  constr_payload_typ: typ;
+  constr_synth: term;
+  constr_synth_recip: branch;
+}
+
+module L = FStar.List.Tot
+
+noextract
+let mk_constr (iname: name) (s: ctor) : Tac constr_t =
+  let (name, typ) = s in
+  let aux = mk_constr_aux iname typ in
+  {
+    constr_payload_typ = aux.constr_aux_payload_typ;
+    constr_synth = (
+      let b = fresh_bv aux.constr_aux_payload_typ in
+      pack (Tv_Abs (mk_binder b) (
+        pack (Tv_Match (pack (Tv_Var b)) [
+          aux.constr_synth_pattern, mk_app (pack (Tv_FVar (pack_fv name))) aux.constr_synth_args
+      ]))))
+    ;
+    constr_synth_recip = (
+      let mp = L.map (fun x -> (Pat_Var x, true)) aux.constr_synth_recip_bvs in
+      Pat_Cons (pack_fv name) mp,
+      aux.constr_synth_recip_body
+    );
+  }
+
+noextract
+let rec mk_maps_aux (iname: name) (c: list ctor) : Tac unit =
+  match c with
+  | [] -> ()
+  | a :: q ->
+    let _ = mk_constr iname a in
+    mk_maps_aux iname q
+
+noextract
+let mk_maps (s: typ) : Tac unit =
+  let (name, ctors) = get_name_and_ctors s in
+  mk_maps_aux name ctors
+
+type t = | A | B of bool
+
+let _ : unit = synth_by_tactic (fun _ ->
+    mk_maps (`t);
+    exact (`())
+  )
+
+(*
+
+let subtype_equals
+  (t0 t1 t2: Type)
+  (x1: t1)
+  (x2: t2)
+: GTot Type0
+= t1 `subtype_of` t0 /\ t2 `subtype_of` t0 /\ ((x1 <: t0) == (x2 <: t0))
+
+noextract
+let rec mk_enum_upto' (x: U8.t) : Tot (list (U8.t & U8.t)) (decreases (U8.v x)) =
+  if x = 0uy
+  then []
+  else
+    let y = x `U8.sub` 1uy in
+    (y, y) :: mk_enum_upto' y
+
+let rec for_all_memb
+  (#a: eqtype)
+  (f: (a -> Tot bool))
+  (l: list a)
+: Lemma
+  (L.for_all f l <==> (forall x . L.mem x l ==> f x))
+= match l with
+  | [] -> ()
+  | _ :: q -> for_all_memb f q
+
+let rec mk_enum_upto_correct
+  (x: U8.t)
+: Lemma
+  (ensures (
+    let l = mk_enum_upto' x in
+    let l1 = L.map fst l in
+    let l2 = L.map snd l in
+    L.noRepeats l1 /\
+    L.noRepeats l2 /\
+    L.for_all (U8.gt x) l1 /\
+    L.for_all (U8.gt x) l2
+  ))
+  (decreases (U8.v x))
+= if x = 0uy
+  then ()
+  else begin
+    let y = x `U8.sub` 1uy in
+    mk_enum_upto_correct y;
+    let l = mk_enum_upto' y in
+    let l1 = L.map fst l in
+    let l2 = L.map snd l in
+    for_all_memb (U8.gt y) l1;
+    for_all_memb (U8.gt y) l2;
+    for_all_memb (U8.gt x) l1;
+    for_all_memb (U8.gt x) l2
+  end
+
+noextract
+let mk_enum_upto (x: U8.t) : Tot (enum U8.t U8.t) =
+  mk_enum_upto_correct x;
+  mk_enum_upto' x
+
+let rec mk_enum_upto_complete
+  (x: U8.t)
+  (y: U8.t)
+: Lemma
+  (requires (U8.v y < U8.v x))
+  (ensures (
+    let l = mk_enum_upto' x in
+    let l1 = L.map fst l in
+    let l2 = L.map snd l in
+    L.mem y l1 /\ L.mem y l2
+  ))
+  (decreases (U8.v x))
+= if U8.v y + 1 = U8.v x
+  then ()
+  else mk_enum_upto_complete (x `U8.sub` 1uy) y
+
+inline_for_extraction
+let mk_enum_upto_key
+  (x: U8.t)
+  (y: U8.t)
+: Pure (enum_key (mk_enum_upto x))
+  (requires (U8.v y < U8.v x))
+  (ensures (fun z -> (z <: U8.t) == y))
+= mk_enum_upto_complete x y;
+  y
+
+inline_for_extraction
+let mk_enum_upto_repr
+  (x: U8.t)
+  (y: U8.t)
+: Pure (enum_repr (mk_enum_upto x))
+  (requires (U8.v y < U8.v x))
+  (ensures (fun z -> (z <: U8.t) == y))
+= mk_enum_upto_complete x y;
+  y
+
+let rec mk_enum_upto_key_repr'
+  (x: U8.t)
+  (y: U8.t)
+: Lemma
+  (requires (U8.v y < U8.v x))
+  (ensures (
+    L.assoc y (mk_enum_upto' x) == Some y
+  ))
+  (decreases (U8.v x))
+= if U8.v y + 1 = U8.v x
+  then ()
+  else mk_enum_upto_key_repr' (x `U8.sub` 1uy) y
+
+let mk_enum_upto_key_repr
+  (x: U8.t)
+  (y: U8.t)
+: Lemma
+  (requires (U8.v y < U8.v x))
+  (ensures (
+    enum_repr_of_key (mk_enum_upto x) (mk_enum_upto_key x y) == mk_enum_upto_repr x y
+  ))
+= mk_enum_upto_key_repr' x y
+
+let mk_enum_upto_repr_key
+  (x: U8.t)
+  (y: U8.t)
+: Lemma
+  (requires (U8.v y < U8.v x))
+  (ensures (
+    enum_key_of_repr (mk_enum_upto x) (mk_enum_upto_repr x y) == mk_enum_upto_key x y
+  ))
+= mk_enum_upto_key_repr x y;
+  enum_key_of_repr_of_key (mk_enum_upto x) (mk_enum_upto_key x y)
+
